First (uncomplete) version of lucas with tree-number

num/Mod_op.v
@@ -13,8 +13,6 @@ Section Mod_op.
  Variable w : Set.
  
  Record mod_op : Set := mk_mod_op {    
-   w0_mod     : w;
-   w1_mod     : w;
    succ_mod   : w -> w;
    add_mod    : w -> w -> w;
    pred_mod   : w -> w;
@@ -106,54 +104,27 @@ Notation "[[ x ]]" :=
  
    Variable m_op : mod_op.
 
-   Variable wf: w -> Prop.
-
    Record mod_spec : Set := mk_mod_spec {
-    (* Basic constructors *)
-      mod_wf_0          : wf w0;
-      mod_wf_spec_1     : wf w1;
-      succ_mod_wf_spec  : 
-                forall w, wf w -> wf (succ_mod m_op w);
-      add_mod_wf_spec   : 
-            forall w1 w2, wf w1 -> wf w2 -> wf (add_mod m_op w1 w2);
-      pred_mod_wf_spec  : 
-                forall w, wf w -> wf (pred_mod m_op w);
-      sub_mod_wf_spec   : 
-            forall w1 w2, wf w1 -> wf w2 -> wf (sub_mod m_op w1 w2);
-      mul_mod_wf_spec   : 
-            forall w1 w2, wf w1 -> wf w2 -> wf (mul_mod m_op w1 w2);
-      square_mod_wf_spec: 
-                forall w, wf w -> wf (square_mod m_op w);
-      power_mod_wf_spec : 
-              forall w p, wf w -> wf (power_mod m_op w p);
-(*
-      shift_wf_spec     :
-              forall w p, wf w -> wf (shift m_op w p);
-      trunc_wf_spec     :
-              forall w p, wf w -> wf (trunc m_op w p);
-*)
-      mod_spec_0        : [|w0|] mod [|b|] = 0;
-      mod_spec_1        : [|w1|] mod [|b|] = 1;
       succ_mod_spec     : 
-                forall w, wf w ->
+                forall w t, [|w|]= t mod [|b|] ->
                           [|succ_mod m_op w|] = ([|w|] + 1) mod [|b|];
       add_mod_spec      :
-            forall w1 w2, wf w1 -> wf w2 ->
+            forall w1 w2 t1 t2, [|w1|]= t1 mod [|b|] -> [|w2|]= t2 mod [|b|] ->
                           [|add_mod m_op w1 w2|] = ([|w1|] + [|w2|]) mod [|b|];
       pred_mod_spec     :
-                forall w, wf w ->
+                forall w t, [|w|]= t mod [|b|] ->
                           [|pred_mod m_op w|] = ([|w|] - 1) mod [|b|];
       sub_mod_spec      :
-            forall w1 w2, wf w1 -> wf w2 ->
+            forall w1 w2 t1 t2, [|w1|]= t1 mod [|b|] -> [|w2|]= t2 mod [|b|] ->
                           [|sub_mod m_op w1 w2|] = ([|w1|] - [|w2|]) mod [|b|];
       mul_mod_spec      :
-            forall w1 w2, wf w1 -> wf w2 ->
+            forall w1 w2 t1 t2, [|w1|]= t1 mod [|b|] -> [|w2|]= t2 mod [|b|] ->
                           [|mul_mod m_op w1 w2|] = ([|w1|] * [|w2|]) mod [|b|];
       square_mod_spec   :
-                forall w, wf w ->
+                forall w t, [|w|]= t mod [|b|] ->
                           [|square_mod m_op w|] = ([|w|] * [|w|]) mod [|b|];
       power_mod_spec    :
-              forall w p, wf w ->
+              forall w t p, [|w|]= t mod [|b|] ->
                           [|power_mod m_op w p|] = (Zpower_pos [|w|] p) mod [|b|]
 (*
       shift_spec        :
@@ -176,8 +147,6 @@ Notation "[[ x ]]" :=
 
  Hint Resolve Zpower_n ZAux.Zmult_lt_0_compat ZPowerAux.Zpower_lt_0.
  
- Let _wf := fun w => [|w|] < [|b|].
-
  Variable op_spec: znz_spec w_op.
 
  Variable m_op : mod_op.
@@ -202,30 +171,6 @@ Notation "[[ x ]]" :=
     (spec_mul op_spec)
     : w_rewrite.
 
- Let _w0_mod := w0.
-
- Lemma _mod_wf_0: _wf _w0_mod.
- unfold _w0_mod, _wf, w0.
- autorewrite with w_rewrite; auto with zarith. 
- Qed.
-
- Lemma _mod_spec_0: [|_w0_mod|] mod [|b|] = 0.
- rewrite Zmod_def_small;
- unfold _w0_mod, w0; autorewrite with w_rewrite; auto with zarith. 
- Qed.
- 
- Let _w1_mod := w1.
-
- Lemma _mod_wf_1: _wf _w1_mod.
- unfold _w1_mod, _wf, w1.
- autorewrite with w_rewrite; auto with zarith. 
- Qed.
-
- Lemma _mod_spec_1: [|_w1_mod|] mod [|b|] = 1.
- rewrite Zmod_def_small;
- unfold _w1_mod, w1; autorewrite with w_rewrite; auto with zarith. 
- Qed.
-
  Let _succ_mod x :=
   let res := without_c (w_succ_c x) in
   match w_compare res b with 
@@ -237,16 +182,8 @@ Notation "[[ x ]]" :=
  unfold znz_to_Z; rewrite <- (spec_0 op_spec); auto.
  Qed.
 
- Lemma _w0_wf : _wf w0.
- unfold _wf; rewrite _w0_is_0; auto with zarith.
- Qed.
-
  Let _w1_is_1: [|w1|] = 1.
  unfold znz_to_Z; rewrite <- (spec_1 op_spec); auto.
- Qed.
-
- Lemma _w1_wf : _wf w1.
- unfold _wf; rewrite _w1_is_1; auto with zarith.
  Qed.
 
  Theorem Zmod_plus_one: forall a1 b1, 0 < b1 -> (a1 + b1) mod b1 = a1 mod b1.
@@ -261,56 +198,37 @@ Notation "[[ x ]]" :=
  apply Zmod_mod; auto.
  Qed.
 
- Lemma _succ_mod_spec: forall w, _wf w ->
+ Lemma without_c_b: forall w2, [|w2|] < [|b|] -> 
+    [|without_c (w_succ_c w2)|] = [|w2|] + 1.
+ intros w2 H.
+ unfold without_c, w_succ_c.
+ generalize (spec_succ_c op_spec w2);  unfold interp_carry; 
+   case (znz_succ_c w_op w2).
+ intros w3 H1; rewrite <- H1; auto with zarith.
+ intros w3; rewrite Zmult_1_l; intros H1.
+ absurd ([|b|] + 1 <= [|w2|] +1); auto with zarith.
+ rewrite <- H1; auto with zarith. 
+ apply Zle_trans with (2 ^ Zpos (znz_digits w_op)); auto with zarith.
+ case (spec_to_Z op_spec b); unfold base; auto with zarith.
+ case (spec_to_Z op_spec w3); unfold base; auto with zarith.
+ Qed.
+
+ Lemma _succ_mod_spec: forall w t, [|w|]= t mod [|b|] ->
     [|_succ_mod w|] = ([|w|] + 1) mod [|b|].
- intros w2; unfold _wf, _succ_mod, w_compare; simpl.
+ intros w2 t H; unfold _succ_mod, w_compare; simpl.
+ assert (F: [|w2|] < [|b|]).
+ case (Z_mod_lt t [|b|]); auto with zarith.
  match goal with |- context[znz_compare _ ?x ?y] =>
    generalize (spec_compare op_spec x y);
    case (znz_compare w_op x y); autorewrite with w_rewrite
  end; try rewrite _w0_is_0; auto with zarith.
- unfold without_c, w_succ_c.
- generalize (spec_succ_c op_spec w2);  unfold interp_carry; 
-   case (znz_succ_c w_op w2).
- intros w3 H H1 H2; rewrite <- H; rewrite H1.
+ rewrite without_c_b; auto with zarith.
+ intros H1; rewrite H1.
  apply sym_equal; apply Z_mod_same; auto with zarith.
- rewrite Zmult_1_l; unfold base.
- intros w3 H H1 H2.
- absurd ([|b|] + 1 <= [|w2|] +1); auto with zarith.
- rewrite <- H; rewrite <- H1; auto with zarith. 
- rewrite (Zplus_comm [|w3|]); apply Zplus_le_compat_r.
- replace 1 with (2 ^ 0); auto with zarith.
- apply ZPowerAux.Zpower_le_monotone; auto with zarith.
- unfold without_c, w_succ_c.
- generalize (spec_succ_c op_spec w2);  unfold interp_carry; 
-   case (znz_succ_c w_op w2).
- intros w3 H H1 H2; rewrite <- H.
- apply sym_equal; apply Zmod_def_small; auto with zarith.
- split; auto.
- case (spec_to_Z op_spec w3); auto.
- rewrite Zmult_1_l; unfold base.
- intros w3 H H1 H2.
- absurd ([|b|] + 1 <= [|w2|] +1); auto with zarith.
- rewrite <- H; auto with zarith. 
- apply Zle_trans with (2 ^ Zpos (znz_digits w_op)); auto with zarith.
- case (spec_to_Z op_spec b); unfold base; auto with zarith.
- case (spec_to_Z op_spec w3); unfold base; auto with zarith.
- unfold without_c, w_succ_c.
- generalize (spec_succ_c op_spec w2);  unfold interp_carry; 
-   case (znz_succ_c w_op w2).
- intros w3 H H1 H2.
- absurd ([|b|] + 1 <= [|w2|] +1); auto with zarith.
- rewrite Zmult_1_l; unfold base.
- intros w3 H H1 H2.
- absurd ([|b|] + 1 <= [|w2|] +1); auto with zarith.
- rewrite <- H; auto with zarith. 
- apply Zle_trans with (2 ^ Zpos (znz_digits w_op)); auto with zarith.
- case (spec_to_Z op_spec b); unfold base; auto with zarith.
- Qed.
-
-
- Lemma _succ_mod_wf_spec: forall w, _wf w -> _wf (_succ_mod w).
- intros w2 Hw2; unfold _wf; rewrite _succ_mod_spec; auto.
- case (Z_mod_lt ([|w2|] + 1) [|b|]); auto with zarith.
+ rewrite without_c_b; auto with zarith.
+ intros H1; rewrite Zmod_def_small; auto with zarith.
+ case (spec_to_Z op_spec w2); auto with zarith.
+ rewrite without_c_b; auto with zarith.
  Qed.
 
  Let split := ww_split w_op.
@@ -326,9 +244,9 @@ Notation "[[ x ]]" :=
   | C1 z => w_add mb z
   end.
 
- Lemma _add_mod_spec: forall w1 w2, _wf w1 -> _wf w2 ->
+ Lemma _add_mod_correct: forall w1 w2, [|w1|] + [|w2|] < 2 * [|b|] ->
      [|_add_mod w1 w2|] = ([|w1|] + [|w2|]) mod [|b|].
- intros w2 w3; unfold _wf, _add_mod, w_compare, w_add_c; intros H H1.
+ intros w2 w3; unfold _add_mod, w_compare, w_add_c; intros H.
  match goal with |- context[znz_add_c _ ?x ?y] =>
    generalize (spec_add_c op_spec x y); unfold interp_carry;
    case (znz_add_c w_op x y); autorewrite with w_rewrite
@@ -343,8 +261,7 @@ Notation "[[ x ]]" :=
  intros H3; rewrite <- H2.
  apply sym_equal; apply Zmod_def_small; auto with zarith.
  case (spec_to_Z op_spec w4); unfold base; auto with zarith.
- intros H3.
- rewrite <- H2.
+ intros H3; rewrite <- H2.
  assert (F1: 0 < [|w4|] - [|b|]); auto with zarith.
  assert (F2: [|w4|] < [|b|] + [|b|]); auto with zarith.
  rewrite (fun x y => Zmod_def_small (x - y)); auto with zarith.
@@ -359,7 +276,10 @@ Notation "[[ x ]]" :=
  assert (F1: [|w4|] < [|b|]).
  assert (F2: base (znz_digits w_op) + [|w4|] < base (znz_digits w_op) + [|b|]);
    auto with zarith.
- case (spec_to_Z op_spec w2); auto with zarith.
+ rewrite H2.
+ apply Zlt_trans with ([|b|] +[|b|]); auto with zarith.
+ apply Zplus_lt_compat_r; auto with zarith.
+ case (spec_to_Z op_spec b); auto with zarith.
  assert (F2: [|b|] < base (znz_digits w_op) + [|w4|]); auto with zarith.
  apply Zlt_le_trans with (base (znz_digits w_op)); auto with zarith.
  case (spec_to_Z op_spec b); auto with zarith.
@@ -379,10 +299,15 @@ Notation "[[ x ]]" :=
  rewrite Zmod_def_small; auto with zarith.
  Qed.
 
- Lemma _add_mod_wf_spec: forall w1 w2, _wf w1 -> _wf w2 -> _wf (_add_mod w1 w2).
- intros w2 w3 H H1.
- unfold _wf; rewrite _add_mod_spec; auto.
- case (Z_mod_lt ([|w2|] + [|w3|]) [|b|]); auto with zarith.
+ Lemma _add_mod_spec: forall w1 w2 t1 t2, [|w1|] = t1 mod [|b|] -> [|w2|] = t2 mod [|b|] ->
+     [|_add_mod w1 w2|] = ([|w1|] + [|w2|]) mod [|b|].
+ intros w2 w3 t1 t2 H H1.
+ apply _add_mod_correct; auto with zarith.
+ assert (F: [|w2|] < [|b|]).
+ case (Z_mod_lt t1 [|b|]); auto with zarith.
+ assert (F': [|w3|] < [|b|]).
+ case (Z_mod_lt t2 [|b|]); auto with zarith.
+ assert (tmp: forall x, 2 * x = x + x); auto with zarith.
  Qed.
 
  Let _pred_mod x :=
@@ -391,18 +316,20 @@ Notation "[[ x ]]" :=
   | _ => without_c (w_pred_c x)
   end.
 
- Lemma _pred_mod_spec: forall w, _wf w ->
+ Lemma _pred_mod_spec: forall w t, [|w|] = t mod [|b|] ->
    [|_pred_mod w|] = ([|w|] - 1) mod [|b|].
- intros w2; unfold _wf, _pred_mod, w_compare, bm1; simpl.
+ intros w2 t H; unfold _pred_mod, w_compare, bm1; simpl.
+ assert (F: [|w2|] < [|b|]).
+ case (Z_mod_lt t [|b|]); auto with zarith.
  match goal with |- context[znz_compare _ ?x ?y] =>
    generalize (spec_compare op_spec x y);
    case (znz_compare w_op x y); autorewrite with w_rewrite
  end; try rewrite _w0_is_0; try rewrite _w1_is_1; auto with zarith.
- intros H H1; rewrite <- H; simpl.
+ intros H1; rewrite <- H1; simpl.
  rewrite <- (Zmod_plus_one (-1)); auto with zarith.
  repeat rewrite Zmod_def_small; auto with zarith.
  case (spec_to_Z op_spec b); auto with zarith.
- intros H1 H2. 
+ intros H1. 
  unfold without_c, w_pred_c.
  generalize (spec_pred_c op_spec w2);  unfold interp_carry; 
    case (znz_pred_c w_op w2).
@@ -415,20 +342,19 @@ Notation "[[ x ]]" :=
  case (spec_to_Z op_spec w2); auto with zarith.
  Qed.
 
- Lemma _pred_mod_wf_spec: forall w, _wf w -> _wf (_pred_mod w).
- intros w2 Hw2; unfold _wf; rewrite _pred_mod_spec; auto.
- case (Z_mod_lt ([|w2|] - 1) [|b|]); auto with zarith.
- Qed.
-
  Let _sub_mod x y :=
   match w_sub_c x y with
   | C0 z => z
   | C1 z => w_add z b
   end.
 
- Lemma _sub_mod_spec: forall w1 w2, _wf w1 -> _wf w2 ->
+ Lemma _sub_mod_spec: forall w1 w2 t1 t2, [|w1|] = t1 mod [|b|] -> [|w2|] = t2 mod [|b|] ->
    [|_sub_mod w1 w2|] = ([|w1|] - [|w2|]) mod [|b|].
- intros w2 w3; unfold _wf, _sub_mod, w_compare, w_sub_c; intros H H1.
+ intros w2 w3 t1 t2; unfold _sub_mod, w_compare, w_sub_c; intros H H1.
+ assert (F: [|w2|] < [|b|]).
+ case (Z_mod_lt t1 [|b|]); auto with zarith.
+ assert (F': [|w3|] < [|b|]).
+ case (Z_mod_lt t2 [|b|]); auto with zarith.
  match goal with |- context[znz_sub_c _ ?x ?y] =>
    generalize (spec_sub_c op_spec x y); unfold interp_carry;
    case (znz_sub_c w_op x y); autorewrite with w_rewrite
@@ -451,13 +377,6 @@ Notation "[[ x ]]" :=
  case (spec_to_Z op_spec b); auto with zarith.
  Qed.
 
- Lemma _sub_mod_wf_spec: forall w1 w2, _wf w1 -> _wf w2 ->
-   _wf (_sub_mod w1 w2).
- intros w2 w3 H H1.
- unfold _wf; rewrite _sub_mod_spec; auto.
- case (Z_mod_lt ([|w2|] - [|w3|]) [|b|]); auto with zarith.
- Qed.
-
  Let _mul_mod x y :=
   let xy := w_mul_c x y in
   match ww_compare w_op xy wwb with
@@ -469,6 +388,19 @@ Notation "[[ x ]]" :=
     let (q,r) := w_div21 h l b2n in
     w_lsr_n r 
   end.
+
+ Theorem high_zero:forall x, [[x]] < base w_digits -> [|fst (split x)|] = 0.
+  intros x; case x; simpl; auto.
+ intros xh xl H; case (Zle_lt_or_eq 0 [|xh|]); auto with zarith.
+ case (spec_to_Z op_spec xh); auto with zarith.
+ intros H1; contradict H; apply Zle_not_lt.
+ unfold base, w_digits; simpl ww_to_Z; unfold base.
+ match goal with |- ?X <= ?Y + ?Z =>
+  pattern X at 1; rewrite <- (Zmult_1_l X); auto with zarith;
+  apply Zle_trans with Y; auto with zarith
+ end.
+ case (spec_to_Z op_spec xl); auto with zarith.
+ Qed.
 
  Theorem n_spec: base (znz_digits w_op) / 2 <= 2 ^ (Z_of_N n) * [|b|] 
                         < base (znz_digits w_op).
@@ -487,7 +419,6 @@ Notation "[[ x ]]" :=
  rewrite (spec_add_mul_div op_spec); auto with zarith.
  rewrite _w0_is_0; rewrite Zdiv_0; auto with zarith.
  rewrite Zplus_0_r; rewrite Zmult_comm; apply Zmod_def_small; auto with zarith.
- split; auto with zarith; red; auto.
  Qed.
 
  Theorem ww_lsl_n_spec: forall w, [[w]] < [|b|] * [|b|] ->
@@ -556,200 +487,95 @@ Notation "[[ x ]]" :=
  split; auto with zarith.
  case p; intros; red; simpl; auto; intros; discriminate.
  rewrite <- U3; rewrite Zdiv_0; auto with zarith.
- split; auto with zarith.
  unfold w_digits; rewrite Zpos_minus; auto with zarith.
  generalize (F p); auto with zarith.
  Qed.
 
- Lemma _mul_mod_spec: forall w1 w2, _wf w1 -> _wf w2 ->
-   [|_mul_mod w1 w2|] = ([|w1|] * [|w2|]) mod [|b|].
- intros w2 w3; unfold _wf, _mul_mod, ww_compare, wwb, w_mul_c; intros H H1.
- match goal with |- context[znz_mul_c _ ?x ?y] =>
-   generalize (spec_mul_c op_spec x y); unfold interp_carry;
-   case (znz_mul_c w_op x y); autorewrite with w_rewrite
- end; auto with zarith.
- match goal with |- context[znz_compare _ ?x ?y] =>
-   generalize (spec_compare op_spec x y);
-   case (znz_compare w_op x y); autorewrite with w_rewrite
- end; try rewrite _w0_is_0; try rewrite _w1_is_1; auto with zarith.
- match goal with |- context[znz_compare
- _ ?x ?y] =>
-   generalize (spec_compare op_spec x y);
-   case (znz_compare w_op x y); autorewrite with w_rewrite
- end; try rewrite _w0_is_0; try rewrite _w1_is_1; auto with zarith.
- intros H2 H3 H4; rewrite <- H4.
- simpl; rewrite (spec_0 op_spec).
- rewrite Zmod_def_small; auto with zarith.
- simpl; intros w4 s5 H2.
- match goal with |- context[znz_compare _ ?x ?y] =>
-   generalize (spec_compare op_spec x y);
-   case (znz_compare w_op x y); autorewrite with w_rewrite
- end; try rewrite _w0_is_0; try rewrite _w1_is_1; auto with zarith.
- intros H3; rewrite <- H2; rewrite H3; simpl.
- match goal with |- context[znz_compare _ ?x ?y] =>
-   generalize (spec_compare op_spec x y);
-   case (znz_compare w_op x y); autorewrite with w_rewrite
- end; try rewrite _w0_is_0; try rewrite _w1_is_1; auto with zarith.
- intros H4; rewrite H4; rewrite Z_mod_same; auto with zarith.
- intros H4; rewrite Zmod_def_small; auto with zarith.
- case (spec_to_Z op_spec s5); auto with zarith.
- rewrite H3 in H2; simpl in H2.
- generalize (ww_lsl_n_spec (WW w4 s5)); 
-  case (ww_lsl_n (WW w4 s5)); auto with arith.
- simpl; rewrite H3; rewrite H2; simpl.
- intros H4 H5; contradict H5; apply Zle_not_gt.
- apply Zmult_le_reg_r with (2 ^ Z_of_N n); auto with zarith.
- rewrite Zmult_comm; rewrite <- H4; auto with zarith.
- apply ZAux.Zmult_lt_compat_bis.
- case (spec_to_Z op_spec w2); auto with zarith.
- case (spec_to_Z op_spec w3); auto with zarith.
- simpl; rewrite H3; rewrite Zmult_0_l; rewrite Zplus_0_l.
- intros w5 w6; simpl; intros H4 H5.
- match type of H4 with ?X -> ?Y =>
-   assert (tmp: X); 
-    [idtac | generalize (H4 tmp); clear tmp H4; intros H4]
- end.
- rewrite H2; apply ZAux.Zmult_lt_compat_bis.
- case (spec_to_Z op_spec w2); auto with zarith.
- case (spec_to_Z op_spec w3); auto with zarith.
- unfold w_div21; generalize (spec_div21 op_spec w5 w6 b2n);
-   case (znz_div21 w_op w5 w6 b2n).
- intros w7 w8 H6; case H6.
- rewrite b2n_spec; case (n_spec); auto.
- rewrite b2n_spec.
- case (Zle_or_lt (2 ^ Z_of_N n * [|b|]) [|w5|]); auto; intros H7.
- match type of H4 with ?X = ?Y =>
-    absurd (Y < X)
- end.
- apply Zle_not_lt; rewrite H4; auto with zarith.
- rewrite H2.
- match goal with |- ?X < ?Y + _ =>
-    apply Zlt_le_trans with Y; auto with zarith
- end.
- rewrite Zmult_assoc; match goal with |- ?X * ?Y < _ =>
-    apply Zle_lt_trans with ([|w5|] * Y); auto with zarith
- end.
- apply Zmult_le_compat_r; auto with zarith.
- case (spec_to_Z op_spec w3); auto with zarith.
- apply Zmult_lt_compat_l; auto with zarith.
- apply Zlt_le_trans with (2 := H7); auto with zarith.
- apply Zlt_trans with [|b|]; auto with zarith.
- case (spec_to_Z op_spec b); auto with zarith.
- case (spec_to_Z op_spec w6); auto with zarith.
- clear H6; rewrite b2n_spec; auto with zarith; intros H6 H7.
- rewrite w_lsr_n_spec; auto with zarith.
- rewrite H6 in H4.
- match type of H4 with ?X * (?Y * ?Z) + ?T = ?Y * ?U =>
-   replace T with (Y * (U - X * Z))
- end; auto with zarith.
- rewrite Zmult_comm; rewrite Z_div_mult; auto with zarith.           
- match goal with |- ?X - ?Y = ?X mod ?T =>
-  apply trans_equal with (((X - Y) + Y) mod T)
- end.
- rewrite Z_mod_plus; auto with zarith.
- apply sym_equal; apply Zmod_def_small; auto with zarith.
- split; auto with zarith.
- apply Zmult_le_reg_r with (2 ^ Z_of_N n); auto with zarith.
- rewrite Zmult_0_l; rewrite Zmult_comm.
- rewrite Zmult_minus_distr_l.
- rewrite <- H4; auto with zarith.
- match goal with |- 0 <= ?X =>
-  replace X with [|w8|]; auto with zarith
- end; ring.
- apply Zmult_lt_reg_r with (2 ^ Z_of_N n); auto with zarith.
- repeat rewrite (fun x y => Zmult_comm x (2 ^y)).
- rewrite Zmult_minus_distr_l.
- rewrite <- H4; auto with zarith.
- match goal with |- ?X < _ =>
-  replace X with [|w8|]; auto with zarith
- end; ring.
- eq_tac; auto with zarith.
- rewrite Zmult_minus_distr_l; rewrite <- H4; auto with zarith.
- ring.
- case (spec_to_Z op_spec w4); auto with zarith.
- intros H3.
- assert (F0: [[WW w4 s5]] < [|b|] * [|b|]).
- simpl; rewrite H2; apply ZAux.Zmult_lt_compat_bis.
- case (spec_to_Z op_spec w2); auto with zarith.
- case (spec_to_Z op_spec w3); auto with zarith.
- generalize (ww_lsl_n_spec (WW w4 s5) F0); clear F0;
-  case (ww_lsl_n (WW w4 s5)); auto with arith.
- simpl.
- intros HH.
- match type of HH with ?Y = ?Z =>
-    absurd (Y < Z)
- end.
- rewrite <- HH; auto with zarith.
- apply ZAux.Zmult_lt_0_compat; auto with zarith.
- match goal with |- ?X < ?Y + ?Z =>
-    apply Zlt_le_trans with Y; auto with zarith
- end.
- apply ZAux.Zmult_lt_0_compat; auto with zarith.
- unfold base; apply ZPowerAux.Zpower_lt_0; auto with zarith.
- case (spec_to_Z op_spec s5); auto with zarith.
- intros w5 w6; simpl; intros H4.
- unfold w_div21; generalize (spec_div21 op_spec w5 w6 b2n);
-   case (znz_div21 w_op w5 w6 b2n).
- intros w7 w8 H6; case H6.
- rewrite b2n_spec; case (n_spec); auto.
- rewrite b2n_spec.
- case (Zle_or_lt (2 ^ Z_of_N n * [|b|]) [|w5|]); auto; intros H7.
- match type of H4 with ?X = ?Y =>
-    absurd (Y < X)
- end.
- apply Zle_not_lt; rewrite H4; auto with zarith.
- rewrite H2.
- match goal with |- ?X < ?Y + _ =>
-    apply Zlt_le_trans with Y; auto with zarith
- end.
- rewrite Zmult_assoc; match goal with |- ?X * ?Y < _ =>
-    apply Zle_lt_trans with ([|w5|] * Y); auto with zarith
- end.
- apply Zmult_le_compat_r; auto with zarith.
- case (spec_to_Z op_spec w3); auto with zarith.
- apply Zmult_lt_compat_l; auto with zarith.
- apply Zlt_le_trans with (2 := H7); auto with zarith.
- apply Zlt_trans with [|b|]; auto with zarith.
- case (spec_to_Z op_spec b); auto with zarith.
- case (spec_to_Z op_spec w6); auto with zarith.
- clear H6; rewrite b2n_spec; auto with zarith; intros H6 H7.
- rewrite w_lsr_n_spec; auto with zarith.
- rewrite H6 in H4.
- match type of H4 with ?X * (?Y * ?Z) + ?T = ?Y * ?U =>
-   replace T with (Y * (U - X * Z))
- end; auto with zarith.
- rewrite Zmult_comm; rewrite Z_div_mult; auto with zarith.           
- rewrite <- H2;
- match goal with |- ?X - ?Y = ?X mod ?T =>
-  apply trans_equal with (((X - Y) + Y) mod T)
- end.
- rewrite Z_mod_plus; auto with zarith.
- apply sym_equal; apply Zmod_def_small; auto with zarith.
- split; auto.
- apply Zmult_le_reg_r with (2 ^ Z_of_N n); auto with zarith.
- rewrite Zmult_0_l; rewrite Zmult_comm.
- rewrite Zmult_minus_distr_l.
- rewrite <- H4; auto with zarith.
- match goal with |- 0 <= ?X =>
-  replace X with [|w8|]; auto with zarith
- end; ring.
- apply Zmult_lt_reg_r with (2 ^ Z_of_N n); auto with zarith.
- repeat rewrite (fun x y => Zmult_comm x (2 ^y)).
- rewrite Zmult_minus_distr_l.
- rewrite <- H4; auto with zarith.
- match goal with |- ?X < _ =>
-  replace X with [|w8|]; auto with zarith
- end; ring.
- eq_tac; auto with zarith.
- rewrite Zmult_minus_distr_l; rewrite <- H4; auto with zarith.
- ring.
- Qed.
+ Lemma split_correct: forall x, let (xh, xl) := split x in [[WW xh xl]] = [[x]].
+ intros x; case x; simpl; autorewrite with w_rewrite; auto with zarith.
+ Qed. 
 
- Lemma _mul_mod_wf_spec: forall w1 w2, _wf w1 -> _wf w2 ->
-   _wf (_mul_mod w1 w2).
- intros w2 w3 H H1.
- unfold _wf; rewrite _mul_mod_spec; auto.
- case (Z_mod_lt ([|w2|] * [|w3|]) [|b|]); auto with zarith.
+ Lemma _mul_mod_spec: forall w1 w2 t1 t2, [|w1|] = t1 mod [|b|] -> [|w2|] = t2 mod [|b|] ->
+   [|_mul_mod w1 w2|] = ([|w1|] * [|w2|]) mod [|b|].
+ intros w2 w3 t1 t2 H H1; unfold _mul_mod, wwb.
+ assert (F: [|w2|] < [|b|]).
+ case (Z_mod_lt t1 [|b|]); auto with zarith.
+ assert (F': [|w3|] < [|b|]).
+ case (Z_mod_lt t2 [|b|]); auto with zarith.
+ match goal with |- context[ww_compare _ ?x ?y] =>
+   generalize (spec_ww_compare op_spec x y);
+   case (ww_compare w_op x y); autorewrite with w_rewrite
+ end; try rewrite _w0_is_0; try rewrite _w1_is_1; auto with zarith.
+ unfold w_mul_c, ww_to_Z; rewrite spec_mul_c; auto with zarith.
+ intros H2; rewrite H2; simpl; rewrite _w0_is_0; rewrite Zmult_0_l;
+   rewrite Zplus_0_l.
+ rewrite Z_mod_same; auto with zarith.
+ generalize (high_zero (w_mul_c w2 w3)).
+ unfold w_mul_c; generalize (spec_mul_c op_spec w2 w3); 
+  case (znz_mul_c w_op w2 w3); simpl; auto with zarith.
+ intros H3 _  _; rewrite <- H3; autorewrite with w_rewrite.
+ rewrite Zmod_def_small; auto with zarith.
+ intros w4 w5; rewrite _w0_is_0; rewrite Zmult_0_l; rewrite Zplus_0_l.
+ intros H2 H3 H4.
+ assert (E1: [|w4|] = 0).
+ apply H3; auto with zarith.
+ apply Zlt_trans with (1 := H4).
+ case (spec_to_Z op_spec b); auto with zarith.
+ generalize H4 H2; rewrite E1; rewrite Zmult_0_l; rewrite Zplus_0_l;
+   clear H4 H2; intros H4 H2.
+ rewrite <- H2; rewrite Zmod_def_small; auto with zarith.
+ case (spec_to_Z op_spec w5); auto with zarith.
+ intros H2.
+ match goal with |- context[split ?x] =>
+ generalize (split_correct x); 
+  case (split x); auto with zarith
+ end.
+ assert (F1: [[w_mul_c w2 w3]] < [|b|] * [|b|]).
+ unfold w_mul_c; rewrite spec_znz_mul_c; auto with zarith.
+ apply ZAux.Zmult_lt_compat_bis; auto with zarith.
+ case (spec_to_Z op_spec w2); auto with zarith.
+ case (spec_to_Z op_spec w3); auto with zarith.
+ intros w4 w5; rewrite ww_lsl_n_spec; auto with zarith.
+ intros H3.
+ unfold w_div21; match goal with |- context[znz_div21 ?x ?y ?z ?t] =>
+   generalize (spec_div21 op_spec y z t);
+   case (znz_div21 x y z t)
+ end.
+ rewrite b2n_spec; case (n_spec); auto.
+ intros H4 H5 w6 w7 H6.
+ case H6; auto with zarith.
+ case (Zle_or_lt (2 ^ Z_of_N n * [|b|]) [|w4|]); auto; intros H7.
+ match type of H3 with ?X = ?Y =>
+    absurd (Y < X)
+ end.
+ apply Zle_not_lt; rewrite H3; auto with zarith.
+ simpl ww_to_Z.
+ match goal with |- ?X < ?Y + _ =>
+    apply Zlt_le_trans with Y; auto with zarith
+ end.
+ apply Zlt_trans with (2 ^ Z_of_N n * ([|b|] * [|b|])); 
+   auto with zarith.
+ apply Zmult_lt_compat_l; auto with zarith.
+ rewrite Zmult_assoc.
+ apply ZAux.Zmult_lt_compat; auto with zarith.
+ case (spec_to_Z op_spec b); auto with zarith.
+ case (spec_to_Z op_spec w5); auto with zarith.
+ clear H6; intros H7 H8.
+ rewrite w_lsr_n_spec; auto with zarith.
+ rewrite <- (Z_div_mult ([|w2|] * [|w3|]) (2 ^ Z_of_N n));
+  auto with zarith; rewrite Zmult_comm.
+ rewrite <- spec_znz_mul_c; auto with zarith.
+ unfold w_mul_c in H3; rewrite <- H3; simpl.
+ rewrite H7; rewrite (fun x => Zmult_comm (2 ^ x));
+   rewrite Zmult_assoc; rewrite Z_div_plus_l; auto with zarith.
+ rewrite Zmod_plus; auto with zarith.
+ rewrite Zmod_mult_0; auto with zarith.
+ rewrite Zplus_0_l; auto with zarith.
+ rewrite Zmod_mod; auto with zarith.
+ rewrite Zmod_def_small; auto with zarith.
+ split; auto with zarith.
+ apply Zdiv_lt_upper_bound; auto with zarith.
+ rewrite Zmult_comm; auto with zarith.
  Qed.
 
  Let _square_mod x :=
@@ -764,183 +590,85 @@ Notation "[[ x ]]" :=
     w_lsr_n r
   end.
 
- Lemma _square_mod_spec: forall w, _wf w ->
+ Lemma _square_mod_spec: forall w t, [|w|] = t mod [|b|] ->
     [|_square_mod w|] = ([|w|] * [|w|]) mod [|b|].
- intros w2; unfold _wf, _square_mod, ww_compare, w_square_c.
- match goal with |- context[znz_square_c _ ?x] =>
-   generalize (spec_square_c op_spec x); unfold interp_carry;
-   case (znz_square_c w_op x); autorewrite with w_rewrite
- end; auto with zarith.
- simpl.
- match goal with |- context[znz_compare _ ?x ?y] =>
-   generalize (spec_compare op_spec x y);
-   case (znz_compare w_op x y); autorewrite with w_rewrite
+ intros w2 t2 H; unfold _square_mod, wwb.
+ assert (F: [|w2|] < [|b|]).
+ case (Z_mod_lt t2 [|b|]); auto with zarith.
+ match goal with |- context[ww_compare _ ?x ?y] =>
+   generalize (spec_ww_compare op_spec x y);
+   case (ww_compare w_op x y); autorewrite with w_rewrite
  end; try rewrite _w0_is_0; try rewrite _w1_is_1; auto with zarith.
- match goal with |- context[znz_compare
- _ ?x ?y] =>
-   generalize (spec_compare op_spec x y);
-   case (znz_compare w_op x y); autorewrite with w_rewrite
- end; try rewrite _w0_is_0; try rewrite _w1_is_1; auto with zarith.
- intros H2 H3 H4 _; rewrite <- H4.
- rewrite Zmod_def_small; auto with zarith.
- simpl; intros w3 s4 H2.
- match goal with |- context[znz_compare _ ?x ?y] =>
-   generalize (spec_compare op_spec x y);
-   case (znz_compare w_op x y); autorewrite with w_rewrite
- end; try rewrite _w0_is_0; try rewrite _w1_is_1; auto with zarith.
- intros H3; rewrite <- H2; rewrite H3; simpl.
- match goal with |- context[znz_compare _ ?x ?y] =>
-   generalize (spec_compare op_spec x y);
-   case (znz_compare w_op x y); autorewrite with w_rewrite
- end; try rewrite _w0_is_0; try rewrite _w1_is_1; auto with zarith.
- intros H4 _; rewrite H4.
+ unfold w_square_c, ww_to_Z; rewrite spec_square_c; auto with zarith.
+ intros H2; rewrite H2; simpl; rewrite _w0_is_0; rewrite Zmult_0_l;
+   rewrite Zplus_0_l.
  rewrite Z_mod_same; auto with zarith.
- intros H4 _; rewrite Zmod_def_small; auto with zarith.
- case (spec_to_Z op_spec s4); auto with zarith.
- rewrite H3 in H2; simpl in H2.
- intros H4 H5.
- assert (F0: [[WW w3 s4]] < [|b|] * [|b|]).
- simpl; rewrite H3; simpl; rewrite H2.
- apply ZAux.Zmult_lt_compat_bis.
- case (spec_to_Z op_spec w2); auto with zarith.
- case (spec_to_Z op_spec w2); auto with zarith.
- generalize (ww_lsl_n_spec (WW w3 s4) F0); clear F0;
-  case (ww_lsl_n (WW w3 s4)); auto with arith.
- simpl; rewrite H3; rewrite H2; simpl; rewrite H2 in H4.
- intros H6; contradict H4; apply Zle_not_gt.
- apply Zmult_le_reg_r with (2 ^ Z_of_N n); auto with zarith.
- rewrite Zmult_comm; rewrite <- H6; auto with zarith.
- simpl; rewrite H3; rewrite Zmult_0_l; rewrite Zplus_0_l.
- intros w4 w5; simpl; intros H6.
- unfold w_div21; generalize (spec_div21 op_spec w4 w5 b2n);
-   case (znz_div21 w_op w4 w5 b2n).
- intros w6 w7 H7; case H7; clear H7.
- rewrite b2n_spec; case (n_spec); auto.
- rewrite b2n_spec.
- apply Zmult_lt_reg_r with (base (znz_digits w_op)); auto with zarith.
- unfold base; auto with zarith.
- match type of H6 with ?X = _ =>
-   apply Zle_lt_trans with X
- end; auto with zarith.
+ generalize (high_zero (w_square_c w2)).
+ unfold w_square_c; generalize (spec_square_c op_spec w2); 
+  case (znz_square_c w_op w2); simpl; auto with zarith.
+ intros H3 _  _; rewrite <- H3; autorewrite with w_rewrite.
+ rewrite Zmod_def_small; auto with zarith.
+ intros w4 w5; rewrite _w0_is_0; rewrite Zmult_0_l; rewrite Zplus_0_l.
+ intros H2 H3 H4.
+ assert (E1: [|w4|] = 0).
+ apply H3; auto with zarith.
+ apply Zlt_trans with (1 := H4).
+ case (spec_to_Z op_spec b); auto with zarith.
+ generalize H4 H2; rewrite E1; rewrite Zmult_0_l; rewrite Zplus_0_l;
+   clear H4 H2; intros H4 H2.
+ rewrite <- H2; rewrite Zmod_def_small; auto with zarith.
  case (spec_to_Z op_spec w5); auto with zarith.
- rewrite H6. 
- rewrite <- Zmult_assoc; apply Zmult_lt_compat_l; auto with zarith.
- simpl; rewrite H2; apply ZAux.Zmult_lt_compat_bis.
- case (spec_to_Z op_spec w2); auto with zarith.
- case (spec_to_Z op_spec w2); auto with zarith.
- rewrite b2n_spec; auto with zarith; intros H7 H8.
- rewrite w_lsr_n_spec; auto with zarith.
- rewrite H7 in H6.
- match type of H6 with ?X * (?Y * ?Z) + ?T = ?Y * ?U =>
-   replace T with (Y * (U - X * Z))
- end; auto with zarith.
- rewrite Zmult_comm; rewrite Z_div_mult; auto with zarith.           
- match goal with |- ?X - ?Y = ?X mod ?T =>
-  apply trans_equal with (((X - Y) + Y) mod T)
+ intros H2.
+ match goal with |- context[split ?x] =>
+ generalize (split_correct x); 
+  case (split x); auto with zarith
  end.
- rewrite Z_mod_plus; auto with zarith.
- apply sym_equal; apply Zmod_def_small; auto with zarith.
- split; auto with zarith.
- apply Zmult_le_reg_r with (2 ^ Z_of_N n); auto with zarith.
- rewrite Zmult_0_l; rewrite Zmult_comm.
- rewrite Zmult_minus_distr_l.
- rewrite <- H6; auto with zarith.
- match goal with |- 0 <= ?X =>
-  replace X with [|w7|]; auto with zarith
- end; ring.
- apply Zmult_lt_reg_r with (2 ^ Z_of_N n); auto with zarith.
- repeat rewrite (fun x y => Zmult_comm x (2 ^y)).
- rewrite Zmult_minus_distr_l.
- rewrite <- H6; auto with zarith.
- match goal with |- ?X < _ =>
-  replace X with [|w7|]; auto with zarith
- end; ring.
- eq_tac; auto with zarith.
- rewrite Zmult_minus_distr_l; rewrite <- H6; auto with zarith.
- ring.
- case (spec_to_Z op_spec w3); auto with zarith.
- intros H3 H4.
- assert (F0: [[WW w3 s4]] < [|b|] * [|b|]).
- simpl; rewrite H2; apply ZAux.Zmult_lt_compat_bis.
+ assert (F1: [[w_square_c w2]] < [|b|] * [|b|]).
+ unfold w_square_c, ww_to_Z; rewrite spec_square_c; auto with zarith.
+ apply ZAux.Zmult_lt_compat_bis; auto with zarith.
  case (spec_to_Z op_spec w2); auto with zarith.
  case (spec_to_Z op_spec w2); auto with zarith.
- generalize (ww_lsl_n_spec (WW w3 s4) F0); clear F0;
-  case (ww_lsl_n (WW w3 s4)); auto with arith.
- simpl.
- intros HH.
- match type of HH with ?Y = ?Z =>
-    absurd (Y < Z)
+ intros w4 w5; rewrite ww_lsl_n_spec; auto with zarith.
+ intros H3.
+ unfold w_div21; match goal with |- context[znz_div21 ?x ?y ?z ?t] =>
+   generalize (spec_div21 op_spec y z t);
+   case (znz_div21 x y z t)
  end.
- rewrite <- HH; auto with zarith.
- apply ZAux.Zmult_lt_0_compat; auto with zarith.
- match goal with |- ?X < ?Y + ?Z =>
-    apply Zlt_le_trans with Y; auto with zarith
- end.
- apply ZAux.Zmult_lt_0_compat; auto with zarith.
- unfold base; apply ZPowerAux.Zpower_lt_0; auto with zarith.
- case (spec_to_Z op_spec s4); auto with zarith.
- intros w4 w5; simpl; intros H5.
- unfold w_div21; generalize (spec_div21 op_spec w4 w5 b2n);
-   case (znz_div21 w_op w4 w5 b2n).
- intros w6 w7 H6; case H6.
  rewrite b2n_spec; case (n_spec); auto.
- rewrite b2n_spec.
+ intros H4 H5 w6 w7 H6.
+ case H6; auto with zarith.
  case (Zle_or_lt (2 ^ Z_of_N n * [|b|]) [|w4|]); auto; intros H7.
- match type of H5 with ?X = ?Y =>
+ match type of H3 with ?X = ?Y =>
     absurd (Y < X)
  end.
- apply Zle_not_lt; rewrite H5; auto with zarith.
- rewrite H2.
+ apply Zle_not_lt; rewrite H3; auto with zarith.
+ simpl ww_to_Z.
  match goal with |- ?X < ?Y + _ =>
     apply Zlt_le_trans with Y; auto with zarith
  end.
- rewrite Zmult_assoc; match goal with |- ?X * ?Y < _ =>
-    apply Zle_lt_trans with ([|w4|] * Y); auto with zarith
- end.
- apply Zmult_le_compat_r; auto with zarith.
- case (spec_to_Z op_spec w2); auto with zarith.
+ apply Zlt_trans with (2 ^ Z_of_N n * ([|b|] * [|b|])); 
+   auto with zarith.
  apply Zmult_lt_compat_l; auto with zarith.
- apply Zlt_le_trans with (2 := H7); auto with zarith.
- case (spec_to_Z op_spec w2); auto with zarith.
+ rewrite Zmult_assoc.
+ apply ZAux.Zmult_lt_compat; auto with zarith.
+ case (spec_to_Z op_spec b); auto with zarith.
  case (spec_to_Z op_spec w5); auto with zarith.
- clear H6; rewrite b2n_spec; auto with zarith; intros H6 H7.
+ clear H6; intros H7 H8.
  rewrite w_lsr_n_spec; auto with zarith.
- rewrite H6 in H5.
- match type of H5 with ?X * (?Y * ?Z) + ?T = ?Y * ?U =>
-   replace T with (Y * (U - X * Z))
- end; auto with zarith.
- rewrite Zmult_comm; rewrite Z_div_mult; auto with zarith.           
- rewrite <- H2;
- match goal with |- ?X - ?Y = ?X mod ?T =>
-  apply trans_equal with (((X - Y) + Y) mod T)
- end.
- rewrite Z_mod_plus; auto with zarith.
- apply sym_equal; apply Zmod_def_small; auto with zarith.
- split; auto.
- apply Zmult_le_reg_r with (2 ^ Z_of_N n); auto with zarith.
- rewrite Zmult_0_l; rewrite Zmult_comm.
- rewrite Zmult_minus_distr_l.
- rewrite <- H5; auto with zarith.
- match goal with |- 0 <= ?X =>
-  replace X with [|w7|]; auto with zarith
- end; ring.
- apply Zmult_lt_reg_r with (2 ^ Z_of_N n); auto with zarith.
- repeat rewrite (fun x y => Zmult_comm x (2 ^y)).
- rewrite Zmult_minus_distr_l.
- rewrite <- H5; auto with zarith.
- match goal with |- ?X < _ =>
-  replace X with [|w7|]; auto with zarith
- end; ring.
- eq_tac; auto with zarith.
- rewrite Zmult_minus_distr_l; rewrite <- H5; auto with zarith.
- ring.
- Qed.
-
- Lemma _square_mod_wf_spec: forall w, _wf w ->
-   _wf (_square_mod w).
- intros w2 H.
- unfold _wf; rewrite _square_mod_spec; auto.
- case (Z_mod_lt ([|w2|] * [|w2|]) [|b|]); auto with zarith.
+ rewrite <- (Z_div_mult ([|w2|] * [|w2|]) (2 ^ Z_of_N n));
+  auto with zarith; rewrite Zmult_comm.
+ rewrite <- spec_square_c; auto with zarith.
+ unfold w_square_c, ww_to_Z in H3; rewrite <- H3; simpl.
+ rewrite H7; rewrite (fun x => Zmult_comm (2 ^ x));
+   rewrite Zmult_assoc; rewrite Z_div_plus_l; auto with zarith.
+ rewrite Zmod_plus; auto with zarith.
+ rewrite Zmod_mult_0; auto with zarith.
+ rewrite Zplus_0_l; auto with zarith.
+ rewrite Zmod_mod; auto with zarith.
+ rewrite Zmod_def_small; auto with zarith.
+ split; auto with zarith.
+ apply Zdiv_lt_upper_bound; auto with zarith.
+ rewrite Zmult_comm; auto with zarith.
  Qed.
 
  Let _power_mod :=
@@ -955,57 +683,42 @@ Notation "[[ x ]]" :=
        _mul_mod (_square_mod pow) x
      end.
 
- Lemma _power_mod_spec: forall w p, _wf w ->
+ Lemma _power_mod_spec: forall w t p, [|w|] = t mod [|b|] ->
    [|_power_mod w p|] = (Zpower_pos [|w|] p) mod [|b|].
- assert(aux: forall w p, _wf w ->
-   [|_power_mod w p|] = (Zpower_pos [|w|] p) mod [|b|] /\ _wf (_power_mod w p)).
- intros w2 p; elim p; simpl; auto with zarith.
+ intros w2 t p; elim p; simpl; auto with zarith.
  intros p' Rec H. 
- case (Rec H); intros Rec1 Rec2; clear Rec.
- match goal with |- ?A /\ ?B =>
-   assert A; try (split; auto)
- end.
+ assert (F: [|w2|] < [|b|]).
+ case (Z_mod_lt t [|b|]); auto with zarith.
  replace (xI p') with (p' + p' + 1)%positive.
  repeat rewrite Zpower_pos_is_exp; auto with zarith.
- rewrite _mul_mod_spec; auto with zarith.
- rewrite _square_mod_spec; auto with zarith.
- rewrite Rec1; auto with zarith.
+ pose (t1 := [|_power_mod w2 p'|]).
+ rewrite _mul_mod_spec with (t1 := t1 * t1)
+                            (t2 := t); auto with zarith.
+ rewrite _square_mod_spec with (t := Zpower_pos [|w2|] p'); auto with zarith.
+ rewrite Rec; auto with zarith.
  assert (tmp: forall p, Zpower_pos p 1 = p); try (rewrite tmp; clear tmp).
  intros p1; unfold Zpower_pos; simpl; ring.
  rewrite <- Zmod_mult; auto with zarith.
  rewrite Zmod_mult; auto with zarith.
  rewrite Zmod_mod; auto with zarith.
  rewrite <- Zmod_mult; auto with zarith.
- apply _square_mod_wf_spec; auto.
+ simpl; unfold t1; apply _square_mod_spec with (t := Zpower_pos [|w2|] p'); auto with zarith.
  rewrite xI_succ_xO; rewrite <- Pplus_diag.
  rewrite Pplus_one_succ_r; auto.
- apply _mul_mod_wf_spec; auto with zarith.
- apply _square_mod_wf_spec; auto with zarith.
  intros p' Rec H. 
- case (Rec H); intros Rec1 Rec2; clear Rec.
- match goal with |- ?A /\ ?B =>
-   assert A; try (split; auto)
- end.
  replace (xO p') with (p' + p')%positive.
  repeat rewrite Zpower_pos_is_exp; auto with zarith.
- rewrite _square_mod_spec; auto with zarith.
- rewrite Rec1; auto with zarith.
+ rewrite _square_mod_spec with (t := Zpower_pos [|w2|] p'); auto with zarith.
+ rewrite Rec; auto with zarith.
  rewrite <- Zmod_mult; auto with zarith.
  rewrite <- Pplus_diag; auto.
- apply _square_mod_wf_spec; auto with zarith.
- intros H; split; auto.
+ intros H.
  assert (tmp: forall p, Zpower_pos p 1 = p); try (rewrite tmp; clear tmp).
  intros p1; unfold Zpower_pos; simpl; ring.
- red in H; rewrite Zmod_def_small; auto with zarith.
+ rewrite Zmod_def_small; auto with zarith.
+ assert (F: [|w2|] < [|b|]).
+ case (Z_mod_lt t [|b|]); auto with zarith.
  case (spec_to_Z op_spec w2); auto with zarith.
- intros w2 p H; case (aux w2 p); auto.
- Qed.
-
- Lemma _power_mod_wf_spec: forall w p, _wf w ->
-   _wf (_power_mod w p).
- intros w2 p H.
- unfold _wf; rewrite _power_mod_spec; auto.
- case (Z_mod_lt (Zpower_pos [|w2|] p) [|b|]); auto with zarith.
  Qed.
 
 (*
@@ -1019,24 +732,12 @@ Notation "[[ x ]]" :=
 
  Definition make_mod_op := 
    mk_mod_op
-     _w0_mod _w1_mod 
      _succ_mod _add_mod 
      _pred_mod _sub_mod
      _mul_mod _square_mod _power_mod.
 
-  Definition new_mod_spec: mod_spec make_mod_op _wf.
+  Definition make_mod_spec: mod_spec make_mod_op.
   apply mk_mod_spec.
-  exact _w0_wf.
-  exact _w1_wf.
-  exact _succ_mod_wf_spec.
-  exact _add_mod_wf_spec.
-  exact _pred_mod_wf_spec.
-  exact _sub_mod_wf_spec.
-  exact _mul_mod_wf_spec.
-  exact _square_mod_wf_spec.
-  exact _power_mod_wf_spec.
-  rewrite _w0_is_0; apply Zmod_def_small; auto with zarith.
-  rewrite _w1_is_1; apply Zmod_def_small; auto with zarith.
   exact _succ_mod_spec.
   exact _add_mod_spec.
   exact _pred_mod_spec.
@@ -1046,5 +747,285 @@ Notation "[[ x ]]" :=
   exact _power_mod_spec.
   Defined.
 
+(*********** Mersenne special **********)
+  
+ Variable p p1: positive.
+
+ Hypothesis p_b: [|b|] = 2 ^ (Zpos p) - 1.
+
+ Hypothesis p_p1: Zpos p + Zpos p1 = Zpos (xO w_digits).
+
+ Hypothesis p_lt_w_digits: Zpos p <= Zpos w_digits.
+
+ Let w_pos_mod := w_op.(znz_pos_mod).
+
+ Let _mmul_mod x y :=
+  let xy := w_mul_c x y in
+  match xy with
+    W0 => w0
+  | WW xh xl =>
+      let xl1 := w_pos_mod p xl in
+        match ww_add_mul_div w_op p1 W0 xy with
+          W0 => match w_compare xl1 b with
+                | Lt => xl1
+                | Eq => w0
+                | Gt => w1
+                end
+        | WW _ xl2 => _add_mod xl1 xl2
+        end
+  end.
+
+ Lemma WW_0: forall x y, [[WW x y]] = 0 -> [|x|] = 0 /\ [|y|] =0.
+ intros x y; simpl; case (spec_to_Z op_spec x); intros H1 H2;
+   case (spec_to_Z op_spec y); intros H3 H4 H5.
+ case Zle_lt_or_eq with (1 := H1); clear H1; intros H1; auto with zarith.
+ absurd (0 < [|x|] * base (znz_digits w_op) + [|y|]); auto with zarith.
+ match goal with |- _ < ?X + _ =>
+  apply Zlt_le_trans with X; auto with zarith
+ end.
+ case Zle_lt_or_eq with (1 := H3); clear H3; intros H3; auto with zarith.
+ absurd (0 < [|x|] * base (znz_digits w_op) + [|y|]); auto with zarith.
+ rewrite <- H1; rewrite Zmult_0_l; auto with zarith.
+ Qed.
+
+ Theorem WW0_is_0: [[W0]] = 0.
+ simpl; auto.
+ Qed.
+  Hint Rewrite WW0_is_0: w_rewrite.
+
+ Theorem mmul_aux0: Zpos (xO w_digits) - Zpos p1 = Zpos p.
+ unfold w_digits.
+ apply trans_equal with (Zpos p + Zpos p1 - Zpos p1); auto with zarith.
+ rewrite p_p1; auto with zarith.
+ Qed.
+
+ Theorem mmul_aux1: 2 ^ Zpos w_digits = 
+     2 ^ (Zpos w_digits - Zpos p) * 2 ^ Zpos p.
+ rewrite <- Zpower_exp; auto with zarith.
+ eq_tac; auto with zarith.
+ Qed.
+
+ Theorem mmul_aux2:forall x,
+   x mod (2 ^ Zpos p - 1) = 
+    ((x / 2 ^ Zpos p) + (x mod 2 ^ Zpos p)) mod (2 ^ Zpos p - 1).
+ intros x; pattern x at 1; rewrite Z_div_mod_eq with (b := 2 ^ Zpos p); auto with zarith.
+ match goal with |- (?X * ?Y + ?Z) mod (?X - 1) = ?T =>
+  replace (X * Y + Z) with (Y * (X - 1) + (Y + Z)); try ring
+ end.
+ rewrite Zmod_plus; auto with zarith.
+ rewrite Zmod_mult_0; auto with zarith; rewrite Zplus_0_l.
+ rewrite Zmod_mod; auto with zarith.
+ Qed.
+
+ Theorem mmul_aux3:forall xh xl,
+   [[WW xh xl]] mod (2 ^ Zpos p) = [|xl|] mod (2 ^ Zpos p).
+ intros xh xl; simpl ww_to_Z; unfold base.
+ rewrite Zmod_plus; auto with zarith.
+ generalize mmul_aux1; unfold w_digits; intros tmp; rewrite tmp;
+   clear tmp. 
+ rewrite Zmult_assoc.
+ rewrite Zmod_mult_0; auto with zarith.
+ rewrite Zplus_0_l; apply Zmod_mod; auto with zarith.
+ Qed.
+
+ Theorem mmul_aux4:forall x,
+  [[x]] < [|b|] * 2 ^  Zpos p ->
+     match ww_add_mul_div w_op p1 W0 x with
+          W0 => 0
+        | WW _ xl2 => [|xl2|]
+     end = [[x]] / 2 ^ Zpos p.
+ intros x Hx.
+ assert (U: Zpos p1 < Zpos (xO (znz_digits w_op))).
+ unfold w_digits in p_p1; rewrite <- p_p1.
+ assert (0 < Zpos p); auto with zarith.
+ red; auto with zarith.
+ assert(U1: [[x]] < 2 ^ (Zpos (xO (znz_digits w_op)) + Zpos p)).
+ apply Zlt_le_trans with (1 := Hx).
+ apply Zle_trans with (2 ^ Zpos p * 2 ^ Zpos p).
+ rewrite p_b; apply Zmult_le_compat_r; auto with zarith.
+ rewrite <- Zpower_exp; auto with zarith.
+ apply ZPowerAux.Zpower_le_monotone; auto with zarith.
+ split; auto with zarith.
+ unfold w_digits in p_p1; rewrite <- p_p1.
+ assert (0 < Zpos p1); auto with zarith.
+ red; simpl; auto.
+ match goal with |- context[ww_add_mul_div ?x ?y ?z ?t] =>
+   generalize (@spec_ww_add_mul_div _ x op_spec z t y U);
+   case (ww_add_mul_div x y z t)
+ end; autorewrite with w_rewrite.
+ rewrite Zmult_0_l; rewrite Zplus_0_l.
+ generalize mmul_aux0; unfold w_digits; intros tmp; rewrite tmp.
+ rewrite Zmod_def_small; auto with zarith.
+ split; auto with zarith.
+ apply Zdiv_pos; auto with zarith.
+ case (spec_ww_to_Z op_spec x); auto with zarith.
+ unfold base.
+ apply Zdiv_lt_upper_bound; auto with zarith.
+ case (spec_ww_to_Z op_spec x); auto with zarith.
+ rewrite <- Zpower_exp; auto with zarith.
+ intros w2 w3; rewrite Zmult_0_l; rewrite Zplus_0_l.
+ generalize mmul_aux0; unfold w_digits; intros tmp; rewrite tmp;
+  clear tmp.
+ simpl ww_to_Z; rewrite Zmod_def_small; auto with zarith.
+ intros H1; 
+   generalize (high_zero (WW w2 w3)); intros tmp;
+   simpl fst in tmp; auto with zarith; 
+   rewrite tmp in H1; clear tmp; auto with zarith.
+ simpl ww_to_Z; rewrite H1; apply Zdiv_lt_upper_bound; auto with zarith.
+ case (spec_ww_to_Z op_spec x); auto with zarith.
+ unfold base; rewrite <- Zpower_exp; auto with zarith.
+ apply Zlt_le_trans with (1 := Hx).
+ apply Zle_trans with (2 ^ Zpos p * 2 ^ Zpos p).
+ rewrite p_b; apply Zmult_le_compat_r; auto with zarith.
+ rewrite <- Zpower_exp; auto with zarith.
+ apply ZPowerAux.Zpower_le_monotone; auto with zarith.
+ split; auto with zarith.
+ apply Zdiv_pos; auto with zarith.
+ case (spec_ww_to_Z op_spec x); auto with zarith.
+ unfold base.
+ apply Zdiv_lt_upper_bound; auto with zarith.
+ case (spec_ww_to_Z op_spec x); auto with zarith.
+ rewrite <- Zpower_exp; auto with zarith.
+ Qed.
+
+ Theorem mmul_aux5:forall xh xl, 
+      [[WW xh xl]] < [|b|] * 2 ^  Zpos p ->
+      let xl1 := w_pos_mod p xl in
+      let r := 
+        match ww_add_mul_div w_op p1 W0 (WW xh xl) with
+          W0 => match w_compare xl1 b with
+                | Lt => xl1
+                | Eq => w0
+                | Gt => w1
+                end
+        | WW _ xl2 => _add_mod xl1 xl2
+        end  in
+        [|r|] = [[WW xh xl]] mod [|b|].
+ intros xh xl Hx xl1 r; unfold r; clear r.
+ generalize (mmul_aux4 _ Hx).
+ assert (U: Zpos p1 < Zpos (xO (znz_digits w_op))).
+ unfold w_digits in p_p1; rewrite <- p_p1.
+ assert (0 < Zpos p); auto with zarith.
+ red; auto with zarith.
+ simpl ww_to_Z; rewrite p_b.
+ rewrite mmul_aux2.
+ match goal with |- context[ww_add_mul_div ?x ?y ?z ?t] =>
+   generalize (@spec_ww_add_mul_div _ x op_spec z t y U);
+   case (ww_add_mul_div x y z t)
+ end; autorewrite with w_rewrite.
+ rewrite Zmult_0_l; rewrite Zplus_0_l.
+ generalize mmul_aux0; unfold w_digits; intros tmp; rewrite tmp; clear tmp.
+ intros H1 H2.
+ rewrite <- H2.
+ rewrite Zplus_0_l.
+ generalize mmul_aux3; simpl ww_to_Z; intros tmp; rewrite tmp; clear tmp;
+   auto with zarith.
+ unfold xl1; unfold w_pos_mod; rewrite <- spec_pos_mod; auto with zarith.
+ unfold w_compare; match goal with |- context[znz_compare _ ?x ?y] =>
+   generalize (spec_compare op_spec x y);
+   case (znz_compare w_op x y); autorewrite with w_rewrite
+ end; try rewrite _w0_is_0; auto with zarith.
+ rewrite <- p_b; intros H3; rewrite H3.
+ rewrite Z_mod_same; auto with zarith.
+ rewrite <- p_b; intros H3; rewrite Zmod_def_small; auto with zarith.
+ case (spec_to_Z op_spec (znz_pos_mod w_op p xl)); unfold w_to_Z; auto with zarith.
+ rewrite p_b; rewrite (spec_pos_mod); auto with zarith.
+ intros H3; assert (HH: [|xl|] mod 2 ^ Zpos p = 2 ^ Zpos p).
+ apply Zle_antisym; auto with zarith.
+ case (Z_mod_lt ([|xl|]) (2 ^ Zpos p)); auto with zarith.
+ rewrite HH.
+ rewrite <- Zmod_minus_one; auto with zarith.
+ rewrite _w1_is_1; rewrite Zmod_def_small; auto with zarith.
+ rewrite Zmult_0_l; rewrite Zplus_0_l.
+ generalize mmul_aux0; unfold w_digits; intros tmp; rewrite tmp; clear tmp.
+ intros w2 w3 H1 H2; rewrite <- H2.
+ generalize mmul_aux3; simpl ww_to_Z; intros tmp; rewrite tmp; clear tmp;
+   auto with zarith.
+ rewrite <- (spec_pos_mod); auto with zarith.
+ unfold xl1; unfold w_pos_mod.
+ rewrite <- p_b; rewrite Zplus_comm.
+ apply _add_mod_correct; auto with zarith.
+ assert (tmp: forall x, 2 * x = x + x); auto with zarith;
+   rewrite tmp; apply Zplus_le_lt_compat; clear tmp; auto with zarith.
+ rewrite spec_pos_mod; auto with zarith.
+ rewrite p_b; case (Z_mod_lt [|xl|] (2 ^ Zpos p)); auto with zarith.
+ rewrite H2; apply Zdiv_lt_upper_bound; auto with zarith.
+ case (spec_ww_to_Z op_spec (WW xh xl)); simpl; auto with zarith.
+ Qed.
+
+ Lemma _mmul_mod_spec: forall w1 w2 t1 t2, [|w1|] = t1 mod [|b|] -> [|w2|] = t2 mod [|b|] ->
+   [|_mmul_mod w1 w2|] = ([|w1|] * [|w2|]) mod [|b|].
+ intros w2 w3 t1 t2; unfold _mmul_mod, w_mul_c; intros H H1.
+ assert (F: [|w2|] < [|b|]).
+ case (Z_mod_lt t1 [|b|]); auto with zarith.
+ assert (F': [|w3|] < [|b|]).
+ case (Z_mod_lt t2 [|b|]); auto with zarith.
+ match goal with |- context[znz_mul_c _ ?x ?y] =>
+   generalize (spec_mul_c op_spec x y); unfold interp_carry;
+   case (znz_mul_c w_op x y); autorewrite with w_rewrite
+ end; auto with zarith.
+ simpl; intros H2; rewrite <- H2; rewrite _w0_is_0; rewrite Zmod_def_small;
+  auto with zarith.
+ intros w4 w5 H2.
+ rewrite mmul_aux5; auto with zarith.
+ rewrite <- H2; auto.
+ unfold ww_to_Z; rewrite H2.
+ apply ZAux.Zmult_lt_compat_bis; auto with zarith.
+ case (spec_to_Z op_spec w2); auto with zarith.
+ case (spec_to_Z op_spec w3); auto with zarith.
+ Qed.
+ Let _msquare_mod x :=
+  let xy := w_square_c x in
+  match xy with
+    W0 => w0
+  | WW xh xl =>
+      let xl1 := w_pos_mod p xl in
+        match ww_add_mul_div w_op p1 W0 xy with
+          W0 =>  match w_compare xl1 b with
+                | Lt => xl1
+                | Eq => w0
+                | Gt => w1
+                end         
+        | WW _ xl2 => _add_mod xl1 xl2
+        end
+  end.
+
+ Lemma _msquare_mod_spec: forall w1 t1, [|w1|] = t1 mod [|b|] -> 
+   [|_msquare_mod w1|] = ([|w1|] * [|w1|]) mod [|b|].
+ intros w2 t2; unfold _msquare_mod, w_square_c; intros H.
+ assert (F: [|w2|] < [|b|]).
+ case (Z_mod_lt t2 [|b|]); auto with zarith.
+ match goal with |- context[znz_square_c _ ?x] =>
+   generalize (spec_square_c op_spec x); unfold interp_carry;
+   case (znz_square_c w_op x); autorewrite with w_rewrite
+ end; auto with zarith.
+ simpl; intros H2; rewrite <- H2; rewrite _w0_is_0; rewrite Zmod_def_small;
+  auto with zarith.
+ intros w4 w5 H2.
+ rewrite mmul_aux5; auto with zarith.
+ rewrite <- H2; auto.
+ unfold ww_to_Z; rewrite H2.
+ apply ZAux.Zmult_lt_compat_bis; auto with zarith.
+ case (spec_to_Z op_spec w2); auto with zarith.
+ case (spec_to_Z op_spec w2); auto with zarith.
+ Qed.
+
+ Definition mmake_mod_op := 
+   mk_mod_op
+     _succ_mod _add_mod 
+     _pred_mod _sub_mod
+     _mmul_mod _msquare_mod _power_mod.
+
+  Definition mmake_mod_spec: mod_spec mmake_mod_op.
+  apply mk_mod_spec.
+  exact _succ_mod_spec.
+  exact _add_mod_spec.
+  exact _pred_mod_spec.
+  exact _sub_mod_spec.
+  exact _mmul_mod_spec.
+  exact _msquare_mod_spec.
+  exact _power_mod_spec.
+  Defined.
+ 
 End Mod_op.
     
